formal/isabelle/ERC_TRUST/TRUST_Runtime_Bridge_Generated.thy
@@ -4,7 +4,7 @@ theory TRUST_Runtime_Bridge_Generated
 begin
 
 definition runtime_bridge_schema_sha256 :: string where
-  "runtime_bridge_schema_sha256 = ''40c15f3716aed0d76369eb0c1d449c93b6990d5f0ad6584d924216a10585a8e2''"
+  "runtime_bridge_schema_sha256 = ''20516f2e63a9cef94da420d65345076c307374cef65c543983de99ea9ae93aaf''"
 
 definition native_runtime_template_sha256 :: string where
   "native_runtime_template_sha256 = ''b82010913d2b6f1f7778c48d05a63e73c7498b62f8829f0ed33a86783c0667c1''"
